execution/tests/DexterTests/DexterGens.v
@@ -1,0 +1,99 @@
+From ConCert Require Import Blockchain LocalBlockchain FA2Token FA2Interface Dexter.
+From ConCert Require Import Serializable.
+From ConCert Require Import LocalBlockchainTests.
+(* From Coq Require Import Morphisms. *)
+From ConCert Require Import Extras.
+From ConCert Require Import Containers.
+From ConCert Require Import BoundedN.
+Global Set Warnings "-extraction-logical-axiom".
+
+From QuickChick Require Import QuickChick. Import QcNotation.
+From ExtLib.Structures Require Import Functor Applicative.
+From ConCert.Execution.QCTests Require Import 
+	ChainGens TestUtils ChainPrinters SerializablePrinters TraceGens DexterPrinters.
+From RecordUpdate Require Import RecordUpdate.
+From Coq Require Import ZArith List.
+Import ListNotations.
+Import RecordSetNotations.
+(* For monad notations *)
+From ExtLib.Structures Require Import Monads.
+Import MonadNotation. Open Scope monad_scope.
+(* Notation "f 'o' g" := (compose f g) (at level 50). *)
+
+Module Type DexterTestsInfo.
+  Parameter fa2_contract_addr : Address.
+  Parameter dexter_contract_addr : Address.
+End DexterTestsInfo.
+
+Module DexterGens (Info : DexterTestsInfo).
+Import Info.
+
+Arguments SerializedValue : clear implicits.
+Arguments deserialize : clear implicits.
+Arguments serialize : clear implicits.
+Definition LocalChainBase : ChainBase := ChainGens.LocalChainBase.
+
+Definition returnGenSome {A : Type} (a : A) := returnGen (Some a).
+
+(* --------------------- FA2 Contract Generators --------------------- *)
+Section DexterContractGens.
+
+Definition gTokensToExchange (balance : N) : G (option N) := 
+  if N.eqb 0%N balance
+  then returnGen None
+  else 
+    amount <- choose (0%N, balance) ;;
+    returnGenSome amount.
+
+Definition gTokenExchange  (state : FA2Token.State) : G (option (Address * Dexter.Msg)):=
+  let has_balance p :=
+    let ledger := snd p in 
+    0 <? FMap.size ledger.(balances) in
+  p <-  (sampleFMapOpt_filter state.(assets) has_balance) ;;
+  let tokenid := fst p in
+  let ledger := snd p in
+  let has_tokens p := N.ltb 0 (snd p) in
+  pp <- sampleFMapOpt_filter ledger.(balances) has_tokens ;;
+  let addr := fst pp in 
+  let nr_tokens : N := snd pp in
+  tokens_to_exchange <- gTokensToExchange nr_tokens ;;
+  let exchange_msg := {|
+    exchange_owner := addr;
+    exchange_token_id := tokenid;
+    tokens_sold := tokens_to_exchange;
+  |} in
+  returnGenSome (addr, other_msg (Dexter.tokens_to_asset exchange_msg))
+.
+
+Definition gDexterAction (lc : LocalChain) : G (option Action) :=
+  let mk_call caller_addr amount msg :=
+		returnGenSome {|
+			act_from := caller_addr;
+			act_body := act_call fa2_contract_addr amount (serialize Dexter.Msg _ msg) 
+    |} in
+  match FMap.find fa2_contract_addr (lc_contract_state_deserialized FA2Token.State lc) with
+  | Some fa2_state => p <- gTokenExchange fa2_state ;;
+                      mk_call (fst p) 0%Z (snd p) 
+  | None => returnGen None
+  end.
+
+End DexterContractGens.
+
+
+Definition gDexterChainTraceList max_acts_per_block lc length := 
+  gLocalChainTraceList_fix lc (fun lc _ => gDexterAction lc) length max_acts_per_block.
+
+(* the '1' fixes nr of actions per block to 1 *)
+Definition token_reachableFrom (lc : LocalChain) pf : Checker := 
+  @reachableFrom AddrSize lc (gDexterChainTraceList 1) pf.
+
+Definition token_reachableFrom_implies_reachable (lc : LocalChain) pf1 pf2 : Checker := 
+  reachableFrom_implies_reachable lc (gDexterChainTraceList 1) pf1 pf2.
+
+End DexterGens.
+
+Module DummyTestInfo <: DexterTestsInfo.
+  Definition fa2_contract_addr := zero_address.
+  Definition dexter_contract_addr := zero_address.
+End DummyTestInfo.
+Module MG := DexterGens.DexterGens DummyTestInfo. Import MG.
