execution/tests/DexterTests/DexterTests.v
@@ -1,0 +1,98 @@
+From ConCert Require Import Blockchain LocalBlockchain FA2Token FA2Interface Dexter.
+From ConCert Require Import Serializable.
+From ConCert Require Import LocalBlockchainTests.
+(* From Coq Require Import Morphisms. *)
+From ConCert Require Import Extras.
+From ConCert Require Import Containers.
+From ConCert Require Import BoundedN.
+Global Set Warnings "-extraction-logical-axiom".
+Require Import ZArith Strings.String.
+
+From QuickChick Require Import QuickChick. Import QcNotation.
+From ExtLib.Structures Require Import Functor Applicative.
+From ConCert.Execution.QCTests Require Import 
+	ChainGens TestUtils ChainPrinters SerializablePrinters TraceGens DexterGens.
+From RecordUpdate Require Import RecordUpdate.
+From Coq Require Import List.
+Import ListNotations.
+Import RecordSetNotations.
+(* For monad notations *)
+From ExtLib.Structures Require Import Monads.
+Import MonadNotation. Open Scope monad_scope.
+Close Scope address_scope.
+(* Notation "f 'o' g" := (compose f g) (at level 50). *)
+
+Definition LocalChainBase : ChainBase := ChainGens.LocalChainBase.
+
+(* the policy which allows both owners and operators to transfer tokens. *)
+Definition policy_all : permissions_descriptor := {|
+  descr_self := self_transfer_permitted;
+  descr_operator := operator_transfer_permitted;
+  descr_sender := owner_no_op;
+  descr_receiver := owner_no_op;
+  descr_custom := None;
+|}.
+
+Definition token_metadata_0 : token_metadata := {|
+  metadata_token_id := 0%N;
+  metadata_decimals := 8%N;
+|}.
+
+Definition token_setup : FA2Token.Setup := {|
+  setup_total_supply := [];
+  setup_tokens := FMap.add 0%N token_metadata_0 FMap.empty; 
+  initial_permission_policy := policy_all;
+|}.
+
+Definition deploy_fa2token : @ActionBody Base := create_deployment 0 FA2Token.contract token_setup.
+Definition fa2_caddr : Address := BoundedN.of_Z_const AddrSize 128%Z.
+
+Definition dexter_setup : Dexter.Setup := {|
+  fa2_caddr_ := fa2_caddr;
+|}.
+
+(* The Dexter contract gets 30 chain assets initially *)
+Definition deploy_dexter : @ActionBody Base := create_deployment 30 Dexter.contract dexter_setup.
+Definition dexter_caddr : Address := BoundedN.of_Z_const AddrSize 129%Z.
+
+Definition chain_with_token_deployed : LocalChain :=  
+  unpack_option (my_add_block lc_initial 
+  [
+    build_act creator (act_transfer person_1 10);
+    build_act creator (act_transfer person_2 10);
+    build_act creator deploy_fa2token;
+    build_act creator deploy_dexter
+  ]).
+
+Definition dexter_other_msg := @other_msg _ DexterMsg _.
+
+
+Definition chain1 : LocalChain :=
+  unpack_option (my_add_block chain_with_token_deployed 
+  [
+    build_act person_1 (act_call fa2_caddr 10%Z (serialize _ _ (msg_create_tokens 0%N))) ;
+    build_act person_2 (act_call fa2_caddr 10%Z (serialize _ _ (msg_create_tokens 0%N)))
+  ]).
+
+Definition dexter_state lc := 
+  match (FMap.find dexter_caddr lc.(lc_contract_state)) with
+  | Some state => deserialize Dexter.State _ state
+  | None => None
+  end.
+Definition token_state lc := 
+  match (FMap.find fa2_caddr lc.(lc_contract_state)) with
+  | Some state => deserialize FA2Token.State _ state
+  | None => None
+  end.
+
+Compute (dexter_state chain1).
+Compute (show (token_state chain1)).
+
+From ConCert.Execution.QCTests Require Import DexterGens.
+
+Module TestInfo <: DexterTestsInfo.
+  Definition fa2_contract_addr := fa2_caddr.
+  Definition dexter_contract_addr := dexter_caddr.
+End TestInfo.
+Module MG := DexterGens.DexterGens TestInfo. Import MG.
+
