execution/tests/SerializablePrinters.v
@@ -1,7 +1,7 @@
 From ConCert Require Import Blockchain LocalBlockchain. 
 From ConCert Require Import Serializable.
 From QuickChick Require Import QuickChick.
-From ConCert.Execution.QCTests Require Import CongressPrinters EIP20TokenPrinters FA2Printers TestContracts.
+From ConCert.Execution.QCTests Require Import CongressPrinters EIP20TokenPrinters FA2Printers TestContracts DexterPrinters.
 
 Local Open Scope string_scope.
 
@@ -12,6 +12,9 @@ Instance showSerializedValue : Show SerializedValue :=
   show v := match @deserialize FA2Token.Msg _ v with
     | Some v => show v
     | None => 
+    match @deserialize Dexter.Msg _ v with
+    | Some v => show v
+    | None =>
     match @deserialize TestContracts.ClientMsg _ v with
     | Some v => show v
     | None =>
@@ -25,6 +28,7 @@ Instance showSerializedValue : Show SerializedValue :=
 		| Some v => show v
 		| None => "<FAILED DESERIALIZATION>" 
 		end
+    end
     end
     end
     end
